Rename except_last -> except_0.

base_logic/derived.v
@@ -12,11 +12,11 @@ Arguments uPred_always_if _ !_ _/.
 Notation "□? p P" := (uPred_always_if p P)
   (at level 20, p at level 0, P at level 20, format "□? p  P").
 
-Definition uPred_except_last {M} (P : uPred M) : uPred M := ▷ False ∨ P.
-Notation "◇ P" := (uPred_except_last P)
+Definition uPred_except_0 {M} (P : uPred M) : uPred M := ▷ False ∨ P.
+Notation "◇ P" := (uPred_except_0 P)
   (at level 20, right associativity) : uPred_scope.
-Instance: Params (@uPred_except_last) 1.
-Typeclasses Opaque uPred_except_last.
+Instance: Params (@uPred_except_0) 1.
+Typeclasses Opaque uPred_except_0.
 
 Class TimelessP {M} (P : uPred M) := timelessP : ▷ P ⊢ ◇ P.
 Arguments timelessP {_} _ {_}.
@@ -547,50 +547,50 @@ Proof. destruct p; simpl; auto using always_later. Qed.
 
 
 (* True now *)
-Global Instance except_last_ne n : Proper (dist n ==> dist n) (@uPred_except_last M).
+Global Instance except_0_ne n : Proper (dist n ==> dist n) (@uPred_except_0 M).
 Proof. solve_proper. Qed.
-Global Instance except_last_proper : Proper ((⊣⊢) ==> (⊣⊢)) (@uPred_except_last M).
+Global Instance except_0_proper : Proper ((⊣⊢) ==> (⊣⊢)) (@uPred_except_0 M).
 Proof. solve_proper. Qed.
-Global Instance except_last_mono' : Proper ((⊢) ==> (⊢)) (@uPred_except_last M).
+Global Instance except_0_mono' : Proper ((⊢) ==> (⊢)) (@uPred_except_0 M).
 Proof. solve_proper. Qed.
-Global Instance except_last_flip_mono' :
-  Proper (flip (⊢) ==> flip (⊢)) (@uPred_except_last M).
+Global Instance except_0_flip_mono' :
+  Proper (flip (⊢) ==> flip (⊢)) (@uPred_except_0 M).
 Proof. solve_proper. Qed.
 
-Lemma except_last_intro P : P ⊢ ◇ P.
-Proof. rewrite /uPred_except_last; auto. Qed.
-Lemma except_last_mono P Q : (P ⊢ Q) → ◇ P ⊢ ◇ Q.
+Lemma except_0_intro P : P ⊢ ◇ P.
+Proof. rewrite /uPred_except_0; auto. Qed.
+Lemma except_0_mono P Q : (P ⊢ Q) → ◇ P ⊢ ◇ Q.
 Proof. by intros ->. Qed.
-Lemma except_last_idemp P : ◇ ◇ P ⊢ ◇ P.
-Proof. rewrite /uPred_except_last; auto. Qed.
+Lemma except_0_idemp P : ◇ ◇ P ⊢ ◇ P.
+Proof. rewrite /uPred_except_0; auto. Qed.
 
-Lemma except_last_True : ◇ True ⊣⊢ True.
-Proof. rewrite /uPred_except_last. apply (anti_symm _); auto. Qed.
-Lemma except_last_or P Q : ◇ (P ∨ Q) ⊣⊢ ◇ P ∨ ◇ Q.
-Proof. rewrite /uPred_except_last. apply (anti_symm _); auto. Qed.
-Lemma except_last_and P Q : ◇ (P ∧ Q) ⊣⊢ ◇ P ∧ ◇ Q.
-Proof. by rewrite /uPred_except_last or_and_l. Qed.
-Lemma except_last_sep P Q : ◇ (P ★ Q) ⊣⊢ ◇ P ★ ◇ Q.
+Lemma except_0_True : ◇ True ⊣⊢ True.
+Proof. rewrite /uPred_except_0. apply (anti_symm _); auto. Qed.
+Lemma except_0_or P Q : ◇ (P ∨ Q) ⊣⊢ ◇ P ∨ ◇ Q.
+Proof. rewrite /uPred_except_0. apply (anti_symm _); auto. Qed.
+Lemma except_0_and P Q : ◇ (P ∧ Q) ⊣⊢ ◇ P ∧ ◇ Q.
+Proof. by rewrite /uPred_except_0 or_and_l. Qed.
+Lemma except_0_sep P Q : ◇ (P ★ Q) ⊣⊢ ◇ P ★ ◇ Q.
 Proof.
-  rewrite /uPred_except_last. apply (anti_symm _).
+  rewrite /uPred_except_0. apply (anti_symm _).
   - apply or_elim; last by auto.
     by rewrite -!or_intro_l -always_pure -always_later -always_sep_dup'.
   - rewrite sep_or_r sep_elim_l sep_or_l; auto.
 Qed.
-Lemma except_last_forall {A} (Φ : A → uPred M) : ◇ (∀ a, Φ a) ⊢ ∀ a, ◇ Φ a.
+Lemma except_0_forall {A} (Φ : A → uPred M) : ◇ (∀ a, Φ a) ⊢ ∀ a, ◇ Φ a.
 Proof. apply forall_intro=> a. by rewrite (forall_elim a). Qed.
-Lemma except_last_exist {A} (Φ : A → uPred M) : (∃ a, ◇ Φ a) ⊢ ◇ ∃ a, Φ a.
+Lemma except_0_exist {A} (Φ : A → uPred M) : (∃ a, ◇ Φ a) ⊢ ◇ ∃ a, Φ a.
 Proof. apply exist_elim=> a. by rewrite (exist_intro a). Qed.
-Lemma except_last_later P : ◇ ▷ P ⊢ ▷ P.
-Proof. by rewrite /uPred_except_last -later_or False_or. Qed.
-Lemma except_last_always P : ◇ □ P ⊣⊢ □ ◇ P.
-Proof. by rewrite /uPred_except_last always_or always_later always_pure. Qed.
-Lemma except_last_always_if p P : ◇ □?p P ⊣⊢ □?p ◇ P.
-Proof. destruct p; simpl; auto using except_last_always. Qed.
-Lemma except_last_frame_l P Q : P ★ ◇ Q ⊢ ◇ (P ★ Q).
-Proof. by rewrite {1}(except_last_intro P) except_last_sep. Qed.
-Lemma except_last_frame_r P Q : ◇ P ★ Q ⊢ ◇ (P ★ Q).
-Proof. by rewrite {1}(except_last_intro Q) except_last_sep. Qed.
+Lemma except_0_later P : ◇ ▷ P ⊢ ▷ P.
+Proof. by rewrite /uPred_except_0 -later_or False_or. Qed.
+Lemma except_0_always P : ◇ □ P ⊣⊢ □ ◇ P.
+Proof. by rewrite /uPred_except_0 always_or always_later always_pure. Qed.
+Lemma except_0_always_if p P : ◇ □?p P ⊣⊢ □?p ◇ P.
+Proof. destruct p; simpl; auto using except_0_always. Qed.
+Lemma except_0_frame_l P Q : P ★ ◇ Q ⊢ ◇ (P ★ Q).
+Proof. by rewrite {1}(except_0_intro P) except_0_sep. Qed.
+Lemma except_0_frame_r P Q : ◇ P ★ Q ⊢ ◇ (P ★ Q).
+Proof. by rewrite {1}(except_0_intro Q) except_0_sep. Qed.
 
 (* Own and valid derived *)
 Lemma always_ownM (a : M) : Persistent a → □ uPred_ownM a ⊣⊢ uPred_ownM a.
@@ -628,9 +628,9 @@ Proof.
   intros; rewrite (bupd_ownM_updateP _ (y =)); last by apply cmra_update_updateP.
   by apply bupd_mono, exist_elim=> y'; apply pure_elim_l=> ->.
 Qed.
-Lemma except_last_bupd P : ◇ (|==> P) ⊢ (|==> ◇ P).
+Lemma except_0_bupd P : ◇ (|==> P) ⊢ (|==> ◇ P).
 Proof.
-  rewrite /uPred_except_last. apply or_elim; auto using bupd_mono.
+  rewrite /uPred_except_0. apply or_elim; auto using bupd_mono.
   by rewrite -bupd_intro -or_intro_l.
 Qed.
 
@@ -643,25 +643,25 @@ Global Instance valid_timeless {A : cmraT} `{CMRADiscrete A} (a : A) :
   TimelessP (✓ a : uPred M)%I.
 Proof. rewrite /TimelessP !discrete_valid. apply (timelessP _). Qed.
 Global Instance and_timeless P Q: TimelessP P → TimelessP Q → TimelessP (P ∧ Q).
-Proof. intros; rewrite /TimelessP except_last_and later_and; auto. Qed.
+Proof. intros; rewrite /TimelessP except_0_and later_and; auto. Qed.
 Global Instance or_timeless P Q : TimelessP P → TimelessP Q → TimelessP (P ∨ Q).
-Proof. intros; rewrite /TimelessP except_last_or later_or; auto. Qed.
+Proof. intros; rewrite /TimelessP except_0_or later_or; auto. Qed.
 Global Instance impl_timeless P Q : TimelessP Q → TimelessP (P → Q).
 Proof.
   rewrite /TimelessP=> HQ. rewrite later_false_excluded_middle.
   apply or_mono, impl_intro_l; first done.
   rewrite -{2}(löb Q); apply impl_intro_l.
-  rewrite HQ /uPred_except_last !and_or_r. apply or_elim; last auto.
+  rewrite HQ /uPred_except_0 !and_or_r. apply or_elim; last auto.
   by rewrite assoc (comm _ _ P) -assoc !impl_elim_r.
 Qed.
 Global Instance sep_timeless P Q: TimelessP P → TimelessP Q → TimelessP (P ★ Q).
-Proof. intros; rewrite /TimelessP except_last_sep later_sep; auto. Qed.
+Proof. intros; rewrite /TimelessP except_0_sep later_sep; auto. Qed.
 Global Instance wand_timeless P Q : TimelessP Q → TimelessP (P -★ Q).
 Proof.
   rewrite /TimelessP=> HQ. rewrite later_false_excluded_middle.
   apply or_mono, wand_intro_l; first done.
   rewrite -{2}(löb Q); apply impl_intro_l.
-  rewrite HQ /uPred_except_last !and_or_r. apply or_elim; last auto.
+  rewrite HQ /uPred_except_0 !and_or_r. apply or_elim; last auto.
   rewrite -(always_pure) -always_later always_and_sep_l'.
   by rewrite assoc (comm _ _ P) -assoc -always_and_sep_l' impl_elim_r wand_elim_r.
 Qed.
@@ -671,18 +671,18 @@ Proof.
   rewrite /TimelessP=> HQ. rewrite later_false_excluded_middle.
   apply or_mono; first done. apply forall_intro=> x.
   rewrite -(löb (Ψ x)); apply impl_intro_l.
-  rewrite HQ /uPred_except_last !and_or_r. apply or_elim; last auto.
+  rewrite HQ /uPred_except_0 !and_or_r. apply or_elim; last auto.
   by rewrite impl_elim_r (forall_elim x).
 Qed.
 Global Instance exist_timeless {A} (Ψ : A → uPred M) :
   (∀ x, TimelessP (Ψ x)) → TimelessP (∃ x, Ψ x).
 Proof.
   rewrite /TimelessP=> ?. rewrite later_exist_false. apply or_elim.
-  - rewrite /uPred_except_last; auto.
+  - rewrite /uPred_except_0; auto.
   - apply exist_elim=> x. rewrite -(exist_intro x); auto.
 Qed.
 Global Instance always_timeless P : TimelessP P → TimelessP (□ P).
-Proof. intros; rewrite /TimelessP except_last_always -always_later; auto. Qed.
+Proof. intros; rewrite /TimelessP except_0_always -always_later; auto. Qed.
 Global Instance always_if_timeless p P : TimelessP P → TimelessP (□?p P).
 Proof. destruct p; apply _. Qed.
 Global Instance eq_timeless {A : cofeT} (a b : A) :
@@ -691,8 +691,8 @@ Proof. intros. rewrite /TimelessP !timeless_eq. apply (timelessP _). Qed.
 Global Instance ownM_timeless (a : M) : Timeless a → TimelessP (uPred_ownM a).
 Proof.
   intros ?. rewrite /TimelessP later_ownM. apply exist_elim=> b.
-  rewrite (timelessP (a≡b)) (except_last_intro (uPred_ownM b)) -except_last_and.
-  apply except_last_mono. rewrite eq_sym.
+  rewrite (timelessP (a≡b)) (except_0_intro (uPred_ownM b)) -except_0_and.
+  apply except_0_mono. rewrite eq_sym.
   apply (eq_rewrite b a (uPred_ownM)); first apply _; auto.
 Qed.
 
